Base and Bernoulli

src/Distributions/Bernoulli/Model.dfy
@@ -7,24 +7,24 @@ include "../../Math/MeasureTheory.dfy"
 include "../../ProbabilisticProgramming/Monad.dfy"
 
 module BernoulliModel {
-  import opened MeasureTheory
-  import opened Monad
+  import MeasureTheory
+  import Monad
 
   // Equation (4.23)
-  function ProbBernoulli(p: Probability): Hurd<bool> {
+  function ProbBernoulli(p: MeasureTheory.Probability): Monad.Hurd<bool> {
     assume {:axiom} false;
     var f :=
       (b: bool) =>
         if b then
           if p <= 0.5 then
-            Return(false)
+            Monad.Return(false)
           else
             ProbBernoulli(2.0 * p - 1.0)
         else
           if p <= 0.5 then
             ProbBernoulli(2.0 * p)
           else
-            Return(true);
-    Bind(Deconstruct, f)
+            Monad.Return(true);
+    Monad.Bind(Monad.Deconstruct, f)
   }
 }
